proofs.v
@@ -1,4 +1,5 @@
 From Coq.Lists Require Import List.
+Require Import ssreflect.
 From istari Require Import source subst_src rules_src help trans.
 From istari Require Import Sigma Tactics
      Syntax Subst SimpSub Promote Hygiene
@@ -8,5 +9,21 @@ Check context.
 Theorem one: forall G D e T ebar w1 l1,
     of_m G e T -> tr D (oof (ppair w1 l1) world) ->
     trans e ebar -> 
-         tr ((gamma_at G (ppair w1 l1)) ++ D) (app ebar (sh (length G) l1))
-            (trans_type T (ppair w1 l1)).
+         tr ((gamma_at G (ppair w1 l1)) ++ D) (oof (app ebar (subst (sh (length G)) l1))
+                                                   (trans_type (ppair w1 l1) T) ).
+  move => G D e T ebar w1 l1 Ds Dtrans.
+  move : w1 l1 Dtrans. induction Ds; intros.
+  10 : {
+    inversion H; subst. simpl.
+    eapply tr_compute; try (
+      apply Relation.star_one; left;
+      eapply reduce_app_beta; try apply reduce_id).
+    4 : {
+      unfold equiv.
+      eapply Relation.star_refl.
+    }
+    4 : { unfold subst1. simpl.
+      unfold equiv.
+    }
+
+  }
